Let the desired vector be $\vec{x}$.  Then, 
\begin{align} 
\myvec{\vec{a}+\vec{b}& \vec{a}-\vec{b}}^\top\vec{x}=0
	\label{eq:12/10/4/2/given}
	\\
	\because 
	\vec{a}+\vec{b}= \myvec{\vec{a} & \vec{b}}\myvec{1 \\ 1}
	\\
	\vec{a} - \vec{b}= \myvec{\vec{a} & \vec{b}}\myvec{1 \\ -1}, 
\end{align}
	\eqref{eq:12/10/4/2/given}
	can be expressed as 
\begin{align}
	\cbrak{\myvec{\vec{a} & \vec{b}}\myvec{1 & 1\\ 1 & -1}}^\top\vec{x}=0\\
\implies 	\myvec{1 & 1\\ 1 & -1}^\top\myvec{\vec{a} & \vec{b}}^\top\vec{x}=0
\\
\implies 	\myvec{1 & 1\\ 1 & -1}\myvec{1 & 1\\ 1 & -1}^\top\myvec{\vec{a} & \vec{b}}^\top\vec{x}=0
\\
	\text{or, }
\myvec{\vec{a} & \vec{b}}^\top\vec{x}=0
\end{align}
which can be expressed as 
\begin{align} 
\myvec{
3&2&2\\
1&2&-2
}
	\xleftrightarrow[R_2 = \frac{R_2}{4}]{R_2=3R_2-R_1}
\myvec{
3&2&2\\
0&1&-2
	}
	\\
	\xleftrightarrow[R_1 = \frac{R_1}{3}]{R_1=R_1 - 2R_2}
\myvec{
1&0&2\\
0&1&-2
}
\end{align}
yielding
\begin{align}
\begin{split}
x_1+2x_3=0\\
x_2-2x_3=0
\end{split}
\implies 
\vec{x}
=x_3\myvec{-2\\2\\1}
\end{align}
Thus, the desired unit vector  is 
\begin{align}
\vec{x}
	=\frac{1}{3}\myvec{-2\\2\\1}
\end{align}
